Lynx.lean
@@ -2,4 +2,5 @@ import Lynx.Term
 import Lynx.Contract
 import Lynx.Modules.Erlang
 import Lynx.Modules.Extensions
+import Lynx.Modules.Erlang.ListLemmas
 import Lynx.Tactic
